%%%%%%%%%%%%%%%%%%%%%%%%%%%%%%%%%%%%%%%%%%%%%%%%%%%%%%%%%%%%%%%%%
% Lecture date: 19-11-05
%%%%%%%%%%%%%%%%%%%%%%%%%%%%%%%%%%%%%%%%%%%%%%%%%%%%%%%%%%%%%%%%%
\chapter{Standard Model}
We will be looking at the gauge group $\SU(2)_\text{L} \times \Uni(1)_\text{Y}$. This will be spontaneously broken into $\Uni(1)_{\text{EM}}$. Strong interaction will add $\SU(3)_\text{C}$ and it doesn't get spontaneously broken.

\section{Leptons}
Reintroduce fermions
\begin{align}
   \psi &= \begin{pmatrix} \chi_\text{L} \\ \eta_\text{R} \end{pmatrix} \\
   \psi_\text{L} &= \begin{pmatrix} \chi_\text{L} \\ 0 \end{pmatrix}
\end{align}
$\SU(2)_\text{L}$ only interacts with $\psi_\text{L}$.

Introduce a doublet
\begin{align}
   L &= \begin{pmatrix} \nu_\text{L} \\ e^-_\text{L} \end{pmatrix} \\
   \nu_\text{L} &= (\psi_\nu)_\text{L} =  \begin{pmatrix} \chi_{\nu \text{L}} \\ 0 \end{pmatrix}    \\
   e_\text{L}^- &= (\psi_{e^-})_\text{L} = \begin{pmatrix} \chi_{e^- \text{L}} \\ 0 \end{pmatrix} \\
   e_\text{L} &= (\psi_e)_\text{L} = \frac{1}{2} \left( \id - \gamma_5 \right) \psi_e \\
   \shortintertext{There is no right-handed neutrino in this theory.}
   R &= e_\text{R} = P_\text{R} (\psi_e) = (\psi_e)_\text{R}
\end{align}

Under $\Uni(1)_\text{Y}$, $\text{L}$ has a charge, $\text{Y} = -1$. $\text{R}$ has a $\Uni(1)_{\text{Y}}$ charge $\text{Y} = -2$.
\begin{align*}
   Q_{\text{EM}} = T^3_\text{L} + \frac{1}{2} Y
\end{align*}
with $T^3_\text{L} = \frac{1}{2} \tau^3$ a generator of $\SU(2)$.

\begin{align*}
   Q_{\text{EM}}(\nu_\text{L}) &= T^3_\text{L}(\nu_\text{L}) + \frac{1}{2} Y(\nu_\text{L}) = \frac{1}{2} - \frac{1}{2} = 0 \\
   Q_{\text{EM}}(e^-_\text{L}) &= T^3_\text{L}(e_\text{L}) + \frac{1}{2} Y(e_\text{L}) = -\frac{1}{2} - \frac{1}{2} = 0 \\
   Q_{\text{EM}}(e^-_\text{R}) &= T^3_\text{L}(e_\text{R}) + \frac{1}{2} Y(e_\text{R}) = 0 - 1 = -1
\end{align*}

\begin{align}
   \comm{T^a}{Y} = 0
\end{align}

Kinetic terms for leptons
\begin{align}
   \lag_{\text{\leptons}}^{\text{kin}} &= \bar{R} i \gamma^\mu D'_\mu R + \bar{L} i \gamma^\mu D_\mu L \\
   D'_\mu &= \partial_\mu + ig' B_\mu \\
   D_\mu &= \partial_\mu + \frac{i}{2} g' B_\mu - ig \frac{\tau^a}{2} W_\mu^a
\end{align}
